Progress on progress theorem

src/ReactorModel/Execution/Progress.lean
@@ -1,7 +1,7 @@
 import ReactorModel.Execution.Trace
-import ReactorModel.Determinism.ExecutionStep
+import ReactorModel.Determinism.Execution
 
-open ReactorType
+open ReactorType Classical
 
 -- TODO: Move the Determinism folder into the Execution folder.
 --       Perhaps also rename it to Theorems, as it contains many lemmas which aren't only relevant
@@ -15,27 +15,77 @@ structure State.Terminal (s : State α) : Prop where
   closed  : s.Closed
   no_next : ∀ g, ¬s.NextTag g
 
-theorem State.Terminal.not_of_not_closed {s : State α} (h : ¬s.Closed) : ¬State.Terminal s :=
+namespace State
+namespace Terminal
+
+variable {s : State α}
+
+theorem not_of_not_closed (h : ¬s.Closed) : ¬State.Terminal s :=
   (h ·.closed)
+
+theorem not_of_next_tag (h : s.NextTag g) : ¬State.Terminal s :=
+  (·.no_next g h)
+
+theorem not_elim (t : ¬s.Terminal) : ¬s.Closed ∨ (∃ g, s.NextTag g) := by
+  by_contra h
+  push_neg at h
+  exact t ⟨h.left, h.right⟩ 
+
+end Terminal
+end State
 
 -- A reactor has the progress property, if from any nonterminal state based at that reactor, we can 
 -- perform an execution step.
 def Progress (rtr : α) : Prop :=
-  ∀ s, (s.rtr = rtr) → ¬s.Terminal → (∃ s', Nonempty $ s ⇓ s')    
+  ∀ s, (s.rtr = rtr) → ¬s.Terminal → (∃ s', s ⇓ s')    
 
-theorem Progress.iff_deps_acyclic {rtr : α} : (Progress rtr) ↔ (Dependency.Acyclic rtr) := by
+namespace Progress
+
+variable {rtr : α}
+
+-- TODO: Factor out a lemma of the form "reactors with no reactions are acyclic."
+theorem to_deps_acyclic_triv (triv : rtr[.rcn] = ∅) (p : Progress rtr) : 
+    Dependency.Acyclic rtr := by
+  simp_all [Dependency.Acyclic.iff_mem_acyclic, triv]
+  intros _ h
+  exact absurd h Partial.not_mem_empty
+
+theorem to_deps_acyclic_nontriv (nontriv : rtr[.rcn].Nonempty) (p : Progress rtr) : 
+    Dependency.Acyclic rtr := by
   simp [Dependency.Acyclic.iff_mem_acyclic]
-  constructor <;> intro h
-  case mp =>
-    intro rcn hm
-    let s : State α := { rtr, tag := 0, progress := ∅ }
-    have hc : ¬s.Closed := sorry -- for nontrivial state: follows from progress = ∅.
-    have ⟨_, ⟨e⟩⟩ := h s rfl (State.Terminal.not_of_not_closed hc)
-    replace e := e.resolve_close hc 
-    exact e.acyclic $ e.progress_empty_mem_rcns_iff rfl |>.mpr hm
-  case mpr =>
-    sorry
-    -- Perhaps you can avoid proving directly that you can perform clearing ports by using a proof by
-    -- contradiction.
+  intro rcn hm
+  let s : State α := { rtr, tag := 0, progress := ∅ }
+  have : s.Nontrivial := ⟨nontriv⟩ 
+  have hc : ¬s.Closed := (Set.not_nonempty_empty ·.progress_Nonempty)
+  have ⟨_, e⟩ := p s rfl (State.Terminal.not_of_not_closed hc)
+  have ⟨e⟩ := e.resolve_close hc 
+  exact e.acyclic $ e.progress_empty_mem_rcns_iff rfl |>.mpr hm
 
+theorem to_deps_acyclic : (Progress rtr) → Dependency.Acyclic rtr :=
+  if h : rtr[.rcn].Nonempty 
+  then to_deps_acyclic_nontriv h 
+  else to_deps_acyclic_triv (Partial.Nonempty.not_to_empty h)
+
+theorem of_deps_acyclic (a : Dependency.Acyclic rtr) : Progress rtr := by
+  intro s hs ht
+  by_cases hc : s.Closed
+  case pos =>
+    have ⟨g, hg⟩ := State.Terminal.not_elim ht |>.resolve_left (not_not.mpr hc)
+    sorry -- by_contra
+    -- Can you avoid proving that you can clear ports by going for proof by contra?
+  case neg =>
+    have : s.Nontrivial := byContradiction (hc $ State.Trivial.of_not_nontrivial · |>.closed)
+    -- This might be the place to break out a lemma that works at the level of instantaneous
+    -- execution steps. On that level you can show that there exists a reaction that doesn't have
+    -- any unprocessed dependencies (assuming the reactor is nontrivial). Then you can show that you
+    -- can create an instantaneous step for that reaction by performing a case distinction on
+    -- whether the reaction is triggered or not - in both cases you can create a step.
+    -- Then you need to show that we can repeat this process for all unprocessed reactions, thus
+    -- obtaining an closed instantaneous execution.
+    sorry
+
+theorem iff_deps_acyclic : (Progress rtr) ↔ (Dependency.Acyclic rtr) :=
+  ⟨to_deps_acyclic, of_deps_acyclic⟩
+
+end Progress
 end Execution
