src/ReactorModel/Execution/Trace.lean
@@ -52,7 +52,7 @@ structure AdvanceTag (s₁ s₂ : State α) where
 
 notation s₁:max " ⇓- " s₂:max => AdvanceTag s₁ s₂
 
-inductive Step (s₁ s₂ : State α)
+inductive Step (s₁ s₂ : State α) : Prop
   | close (h : s₁ ⇓| s₂)
   | advance (h : s₁ ⇓- s₂)
 
@@ -62,7 +62,7 @@ end Execution
 
 open Execution
 
-inductive Execution : State α → State α → Type
+inductive Execution : State α → State α → Prop
   | refl : Execution s s
   | step : (s₁ ⇓ s₂) → (Execution s₂ s₃) → Execution s₁ s₃
 
